\chapter{Weighted \v{C}ech complex can be represented as a GDF}
\label{app:weighted_cech}

\begin{lemma}
    For any point cloud $P \subseteq \R^d$, a function $g : P \to \R_{\geq 0}$, and a
    parameter $q \in [1, \infty)$, the weighted \v{C}ech filtration
    $V^a_q[P, g]$ is equal to the sublevel set of the generalised density
    function
    \begin{equation}
        f_{g, q}(P, x) = \min_{p \in P} (d(x, p)^q + g(p)^q)^{1/q}.
    \end{equation}
\end{lemma}

\begin{proof}
    Fix $P, g, q$, and $a$. A point $x \in \R^d$ being included in $V^a_q[P, g]$
    is equivalent to the condition
    \begin{equation}
        \exists p \in P : d(x, p) \leq r_p^{(q)}(a).
    \end{equation}
    Suppose $a \geq g(p)$. Then, we have two cases:
    \begin{enumerate}
        \item $q = \infty$. Then, the condition is equivalent to
            \begin{equation}
                \exists p \in P : d(x, p) \leq a.
            \end{equation}
            The proposed GDF takes value
            \begin{equation}
                f_{g, q}(P, x) = \min_{p \in P} \max(d(x, p), g(p)),
            \end{equation}
            and the sublevel set $f^{-1}_{g, q, P}(-\infty, a]$ is precisely
            \begin{equation}
                \{x \in \R^d \mid \exists p \in P : \max(d(x, p), g(p)) \leq a\},
            \end{equation}
            which, due to $a \geq g(p)$, is the set
            \begin{equation}
                \{x \in \R^d \mid \exists p \in P : d(x, p) \leq a\},
            \end{equation}
            which is the same as $V^a_\infty[P, g]$.
        \item $q < \infty$. Then, the condition is equivalent to
            \begin{equation}
                \exists p \in P : d(x, p) \leq (a^q - g(p)^q)^{1/q}
            \end{equation}
            The proposed GDF takes value
            \begin{equation}
                f_{g, q}(P, x) = \min_{p \in P} (d(x, p)^q + g(p)^q)^{1/q},
            \end{equation}
            and the sublevel set $f^{-1}_{g, q, P}(-\infty, a]$ is precisely
            \begin{equation}
                \{x \in \R^d \mid \exists p \in P : (d(x, p)^q + g(p)^q)^{1/q} \leq a\},
            \end{equation}
            which can be seen to be the same with trivial algebraic manipulations:
            \begin{align}
                (d(x, p)^q + g(p)^q)^{1/q} & \leq a \\
                d(x, p)^q + g(p)^q & \leq a^q \\
                d(x, p)^q & \leq a^q - g(p)^q\\
                d(x, p) & \leq (a^q - g(p)^q)^{1 / q}
            \end{align}
    \end{enumerate}

    Now suppose $a < g(p)$. Then $r_p^{(q)}(a) = - \infty$, and thus the balls
    contain no points. As $(d(x, p)^q + g(p)^q)^{1/q} \geq g(p) > a$, the sublevel
    set is also empty.
\end{proof}

\chapter{The generalised \v{C}ech complex using the Mahalanobis distance kernel is stable}
\label{app:mahalanobis}

\begin{lemma}
    The generalised \v{C}ech complex using the Mahalanobis distance kernel
    \begin{equation}
        h(x, p, P) = \sqrt{(x - p)^\top (\Sigma(p, P) + \varepsilon I)^{-1} (x - p)} = \norm{A(p, P) (x - p)}_2,
    \end{equation}
    where $A(p, P) = (\Sigma(p, P) + \varepsilon I)^{-1/2}$ is stable.
\end{lemma}
\begin{proof}
    To use Theorem~\ref{thm:pc_kernel_stability}, we need to bound
    $|h(x, p, P) - h(x, q, P)|$ and $|h(x, p, P) - h(x, p, Q)|$.
    Bounding the first term, we have:
    \begin{align}
        & |h(x, p, P) - h(x, q, P)| \nonumber \\
        & = |\norm{A(p, P) (x - p)}_2 - \norm{A(q, P) (x - q)}_2| \\
        & \leq \norm{A(p, P) (x - p) - A(q, P) (x - q)}_2 \\
        & = \norm{A(p, P) (x - p) - A(q, P) (x - q) + A(p, P)(x - q) - A(p, P)(x - q)}_2 \\
        & = \norm{A(p, P) (q - p) + (A(p, P) - A(q, P))(x - q)}_2 \\
        & \leq \norm{A(p, P)(q - p)}_2 + \norm{(A(p, P) - A(q, P))(x - q)}_2 \\
        & \leq \norm{A(p, P)}_{\mathrm{op}} \cdot \norm{q - p}_2 + \norm{A(p, P) - A(q, P)}_{\mathrm{op}} \cdot \norm{x - q}_2. \label{eq:bound_h_diff}
    \end{align}
    The operator norm $\norm{A(p, P)}_{\mathrm{op}} = \sup_{v : \norm{v}_2 = 1}
    \norm{A(p, P)v}_2$ is precisely the largest eigenvalue of the matrix $A(p, P)$. 
    As $\Sigma(p, P)$ is positive semi-definite, adding it to $\varepsilon I$ cannot
    decrease the eigenvalues, and thus
    $\norm{\Sigma(p, P) + \varepsilon I}_{\mathrm{op}} \geq \varepsilon$, which implies
    \begin{equation}
        \norm{A(p, P)}_{\mathrm{op}} \leq \varepsilon^{-1/2}.
    \end{equation}
    We now bound the second term, $\norm{A(p, P) - A(q, P)}_{\mathrm{op}}$.
    First we bound $\norm{A(p, P) - A(q, P)}_{\mathrm{op}}$ in terms of
    $\norm{\Sigma(p, P) - \Sigma(q, P)}_{\mathrm{op}}$.
    As $(\Sigma(p, P) + \varepsilon I)$ is positive definite for $\varepsilon > 0$,
    we can represent $A = (\Sigma + \varepsilon I)^{-1/2}$ as an integral:
    \begin{equation}
        (\Sigma + \varepsilon I)^{-1/2} = \frac{1}{\pi} \int_0^\infty t^{-1/2} (\Sigma + (\varepsilon + t)I)^{-1} \dd{t}.
    \end{equation}
    Using the identity $A^{-1} - B^{-1} = A^{-1}(B - A)B^{-1}$, we get:
    \begin{align}
        & A(p, P) - A(q, P) \nonumber \\
        & = \frac{1}{\pi} \int_0^\infty t^{-1/2} \frac{\Sigma(p, P) - \Sigma(q, P)}{(\Sigma(p, P) + (\varepsilon + t)I) (\Sigma(q, P) + (\varepsilon + t)I)} \dd{t}.
    \end{align}
    Taking the operator norm and using $\norm{\Sigma + (\varepsilon + t)I}_{\mathrm{op}} \geq \varepsilon + t$, we have:
    \begin{align}
        & ||A(p, P) - A(q, P)||_{\mathrm{op}} \nonumber \\
        & \leq \frac{1}{\pi} \int_0^\infty t^{-1/2} \norm{\Sigma(p, P) - \Sigma(q, P)}_{\mathrm{op}} \cdot (\varepsilon + t)^{-1} \cdot (\varepsilon + t)^{-1} \dd{t} \\
        & = \frac{1}{\pi} \norm{\Sigma(p, P) - \Sigma(q, P)}_{\mathrm{op}} \int_0^\infty t^{-1/2} (\varepsilon + t)^{-2} \dd{t} \\
        & = \norm{\Sigma(p, P) - \Sigma(q, P)}_{\mathrm{op}} \frac{1}{2} \varepsilon^{-3/2}.
    \end{align}
    Now we bound $\norm{\Sigma(p, P) - \Sigma(q, P)}_{\mathrm{op}}$.
    We can split the term $k(\Sigma(p, P) - \Sigma(q, P))$ into three sums:
    \begin{align}
        & k(\Sigma(p, P) - \Sigma(q, P)) \nonumber \\
        & = \sum_{x \in N_k(p, P) \cap N_k(q, P)}[(x - p)(x - p)^\top - (x - q)(x - q)^\top] + \nonumber \\
        & \sum_{x \in N_k(p, P) \setminus N_k(q, P)} (x - p)(x - p)^\top +
        \sum_{x \in N_k(q, P) \setminus N_k(p, P)} (x - q)(x - q)^\top.
    \end{align}
    The first term is bounded by
    \begin{equation}
        \sum_{x \in N_k(p, P) \cap N_k(q, P)} 2\norm{x - p}_2 \norm{p - q}_2 + \norm{p - q}_2^2 \leq k(2R_p \cdot d_H + d_H^2),
    \end{equation}
    where $R_p$ is the radius of the $k$-neighbourhood of $p$ and $d_H = d_H(P, Q)$.
    
    The other two terms are bounded by $k R_p^2$ and $k R_q^2$, respectively.

    Combining these bounds, we have:
    \begin{equation}
        \norm{\Sigma(p, P) - \Sigma(q, P)}_{\mathrm{op}} \leq 2R_p \cdot d_H + d_H^2 + R_p^2 + R_q^2,
    \end{equation}
    and combining this with the bound of $\norm{A(p, P) - A(q, P)}_{\mathrm{op}}$, we get:
    \begin{equation}
        \norm{A(p, P) - A(q, P)}_{\mathrm{op}} \leq \frac{1}{2} \varepsilon^{-3/2} (2R_p \cdot d_H + d_H^2 + R_p^2 + R_q^2).
    \end{equation}
    Finally, plugging this into
    Equation~\eqref{eq:bound_h_diff}, we have:
    \begin{equation}
        |h(x, p, P) - h(x, q, P)| \leq \varepsilon^{-1/2} d_H + \frac{1}{2} \varepsilon^{-3/2} (2R_p \cdot d_H + d_H^2 + R_p^2 + R_q^2) \cdot R_q.
    \end{equation}
    
    Via similar reasoning, we can bound $|h(x, p, P) - h(x, p, Q)$:
    \begin{align}
        |h(x, p, P) - h(x, p, Q)| & = |||\norm{A(p, P) (x - p)}_2 - \norm{A(p, Q) (x - p)}_2| \\
        & \leq \norm{A(p, P) (x - p) - A(p, Q) (x - p)}_2 \\
        & = \norm{(A(p, P) - A(p, Q)) (x - p)}_2 \\
        & \leq \norm{A(p, P) - A(p, Q)}_{\mathrm{op}} \cdot \norm{x - p}_2 \\
        & \leq \frac{1}{2} \varepsilon^{-3/2} d_H \cdot (R_p^2 + R_q^2) \cdot R_p.
    \end{align}

    By choosing a sufficiently large $\varepsilon$, we achieve the bounds needed
    by Theorem~\ref{thm:pc_kernel_stability}.
\end{proof}
